src/vgtrans.ml
@@ -4,7 +4,4 @@ let _ =
   let prefix = Sys.argv.(1) in
   let (f, tdb(*, db*)) = parse prefix in
   let _ = vgtrans (prefix ^ ".v") tdb (*db *)f in
-  let _ =
-    (let ch = open_out (prefix ^ ".mfotl") in
-     Printf.fprintf ch "%s\n" (mfotl_of_fmla f); close_out ch) in
   ()
