tools/db.h
@@ -1,0 +1,141 @@
+#ifndef __LOG_H__
+#define __LOG_H__
+
+#include <cassert>
+#include <climits>
+#include <map>
+#include <set>
+#include <sstream>
+#include <string>
+#include <vector>
+
+static int let(char c) {
+    return ('A' <= c && c <= 'Z') || ('a' <= c && c <= 'z');
+}
+
+static int num(char c) {
+    return ('0' <= c && c <= '9');
+}
+
+static int anum(char c) {
+    return let(c) || num(c);
+}
+
+static int ws(char c) {
+    return c == ' ' || c == '\n' || c == '\r';
+}
+
+std::map<std::string, std::vector<std::vector<int> > > parse_db(const char *db_buf, size_t db_len) {
+    std::map<std::string, std::vector<std::vector<int> > > res;
+    size_t pos = 0;
+    while (pos < db_len && db_len != -1) {
+        while (pos < db_len && ws(db_buf[pos])) pos++;
+        if (pos == db_len) break;
+        if (!let(db_buf[pos])) throw std::runtime_error("corrupted database");
+        std::string name;
+        while (pos < db_len && anum(db_buf[pos])) name.push_back(db_buf[pos++]);
+        while (pos < db_len && ws(db_buf[pos])) pos++;
+        if (pos == db_len || db_buf[pos] != '(') throw std::runtime_error("corrupted database");
+        pos++;
+        std::vector<int> tuple;
+        while (pos < db_len && db_buf[pos] != ')') {
+            while (pos < db_len && ws(db_buf[pos])) pos++;
+            if (pos < db_len && db_buf[pos] == ')') break;
+            if (!num(db_buf[pos])) throw std::runtime_error("corrupted database");
+            std::string tmp;
+            while (pos < db_len && num(db_buf[pos])) tmp.push_back(db_buf[pos++]);
+            errno = 0;
+            long n = strtol (tmp.c_str(), NULL, 10);
+            if (!(INT_MIN <= n && n <= INT_MAX && errno != ERANGE)) throw std::runtime_error("corrupted database");
+            tuple.push_back(n);
+            while (pos < db_len && ws(db_buf[pos])) pos++;
+            if (pos < db_len && db_buf[pos] == ')') break;
+            if (pos == db_len || db_buf[pos] != ',') throw std::runtime_error("corrupted database");
+            pos++;
+        }
+        res[name].push_back(tuple);
+        if (pos < db_len) pos++;
+    }
+    return res;
+}
+
+FILE *open_file_type(const char *prefix, const char *ftype, const char *mode) {
+    std::ostringstream oss;
+    oss << prefix << ftype;
+    return fopen(oss.str().c_str(), mode);
+}
+
+void dump_db(const char *base, std::map<std::string, std::vector<std::vector<int> > > db, int sql_insert = 0) {
+    FILE *psql = open_file_type(base, ".psql", "w");
+    FILE *msql = open_file_type(base, ".msql", "w");
+    FILE *radb = open_file_type(base, ".radb", "w");
+    fprintf(psql, "DROP TABLE IF EXISTS tbl_T;\n");
+    fprintf(psql, "CREATE TABLE tbl_T (t INT);\n");
+    fprintf(psql, "INSERT INTO tbl_T VALUES (1);\n");
+    fprintf(msql, "USE db;\n");
+    fprintf(msql, "DROP TABLE IF EXISTS tbl_T;\n");
+    fprintf(msql, "CREATE TABLE tbl_T (t INT);\n");
+    fprintf(msql, "INSERT INTO tbl_T VALUES (1);\n");
+    fprintf(radb, "\\sqlexec_{DROP TABLE IF EXISTS tbl_T};\n");
+    fprintf(radb, "\\sqlexec_{CREATE TABLE tbl_T (t INT)};\n");
+    fprintf(radb, "\\sqlexec_{INSERT INTO tbl_T VALUES (1)};\n");
+    for (std::map<std::string, std::vector<std::vector<int> > >::iterator sig = db.begin(); sig != db.end(); sig++) {
+        const char *name = sig->first.c_str();
+        assert(sig->second.size() != 0);
+        int n = sig->second[0].size();
+        fprintf(psql, "DROP TABLE IF EXISTS tbl_%s;\n", name);
+        fprintf(psql, "CREATE TABLE tbl_%s (", name);
+        fprintf(msql, "DROP TABLE IF EXISTS tbl_%s;\n", name);
+        fprintf(msql, "CREATE TABLE tbl_%s (", name);
+        fprintf(radb, "\\sqlexec_{DROP TABLE IF EXISTS tbl_%s};\n", name);
+        fprintf(radb, "\\sqlexec_{CREATE TABLE tbl_%s (", name);
+        const char *sep = "";
+        for (int i = 0; i < n; i++) {
+          fprintf(psql, "%sx%d INT", sep, i);
+          fprintf(msql, "%sx%d INT", sep, i);
+          fprintf(radb, "%sx%d INT", sep, i);
+          sep = ", ";
+        }
+        fprintf(psql, ");\n");
+        fprintf(msql, ");\n");
+        fprintf(radb, ")};\n");
+        if (!sql_insert) {
+          fprintf(psql, "COPY tbl_%s FROM '%s_%s.csv' DELIMITER ',' CSV;\n", name, base, name);
+          fprintf(msql, "LOAD DATA LOCAL INFILE '%s_%s.csv' INTO TABLE tbl_%s FIELDS TERMINATED BY ',';\n", base, name, name);
+        }
+        std::ostringstream oss;
+        oss << base << "_" << name << ".csv";
+        FILE *tbl = fopen(oss.str().c_str(), "w");
+        for (auto it : sig->second) {
+          int _n = it.size();
+          assert(n == _n);
+          if (sql_insert) {
+            fprintf(psql, "INSERT INTO tbl_%s VALUES (", name);
+            fprintf(msql, "INSERT INTO tbl_%s VALUES (", name);
+            fprintf(radb, "\\sqlexec_{INSERT INTO tbl_%s VALUES (", name);
+          }
+          const char *sep2 = "";
+          for (int j = 0; j < n; j++) {
+              fprintf(tbl, "%s%d", sep2, it[j]);
+              if (sql_insert) {
+                fprintf(psql, "%s%d", sep2, it[j]);
+                fprintf(msql, "%s%d", sep2, it[j]);
+                fprintf(radb, "%s%d", sep2, it[j]);
+              }
+              sep2 = ",";
+          }
+          fprintf(tbl, "\n");
+          if (sql_insert) {
+            fprintf(psql, ");\n");
+            fprintf(msql, ");\n");
+            fprintf(radb, ")};\n");
+          }
+        }
+        fclose(tbl);
+    }
+    fclose(psql);
+    fclose(msql);
+    fclose(radb);
+}
+
+#endif
