tools/db2csv.cpp
@@ -1,0 +1,20 @@
+#include "db.h"
+
+#include <cstdio>
+#include <string>
+
+int main(int argc, char **argv)
+{
+  FILE *db_file = open_file_type(argv[1], ".db", "r");
+  char *db_buf = NULL;
+  size_t db_buf_len = 0;
+  size_t db_len = getline(&db_buf, &db_buf_len, db_file);
+  fclose(db_file);
+
+  std::map<std::string, std::vector<std::vector<int> > > db = parse_db(db_buf, db_len);
+  free(db_buf);
+
+  dump_db(argv[1], db, 0);
+
+  return 0;
+}
