README.md
@@ -1,6 +1,4 @@
-This repository is the supplementary material for the paper
-
-Practical Relational Calculus Query Evaluation
+# RC2SQL
 
 RC2SQL is a tool for translating relational calculus (RC) queries to SQL.
 RC2SQL takes as input a RC query and a training database
@@ -8,13 +6,23 @@ and outputs a pair of RANF queries:
 - one characterizing the query's relative safety
 - and one equivalent to the query if the query is relatively safe.
 
+The training database is only used by heuristics in query translation.
+The choice of a training database does NOT impact the translation's correctness.
+
 VGTrans is our implementation of the translation by Van Gelder & Topor.
 VGTrans has the same interface as RC2SQL.
+
+This repository is the supplementary material for the paper
+
+Practical Relational Calculus Query Evaluation
+
+accepted at ICDT'22.
 
 ---
 
 # News:
 
+- December 19: added press-the-button scripts for RC query evaluation
 - September 23: the evaluation results have been updated (see `paper.pdf`)
   after an optimization in the translation of RA expressions to SQL
   (replacing `COUNT(DISTINCT ...)` by `COUNT(...)` and using `SELECT DISTINCT ...`)
@@ -25,22 +33,23 @@ VGTrans has the same interface as RC2SQL.
 
 - `paper.pdf` - paper on RC2SQL
 - `Dockerfile` - Dockerfile for this supplementary material
-- `run_tests.sh` - script to run correctness tests
-- `run.sh` - script to run the experiments
+- `test_all.sh` - script to run correctness tests of query evaluation
+- `run.sh` - script to run experiments
 - `bold.*` - scripts for postprocessing evaluation results (e.g., highlighting fastest execution)
 - `main.tex` - template of a LaTeX document with evaluation results
-- `exps*.sh` - scripts for the individual experiments
-- `rw*.sh` - scripts invoking a database engine to evaluate a pair of queries
-after translation
+- `exps_*.sh` - scripts to run the individual experiments
+- `eval_*.sh` - scripts evaluating an RC query using RC2SQL and a given database engine
+- `run_*.sh` - scripts invoking a database engine to evaluate a pair of queries after translation
 - `mpreg.sh` - script evaluating a query using MonPoly-REG
-- `radb.sh` - script for the translation from relational algebra (RA) to SQL
-- `test_rw.sh` - script to test our translation and the implementation of VGTrans
+- `radb.sh` - script translating relational algebra (RA) to SQL
+- `test_eval.sh` - script to test our translation and the implementation of VGTrans
 against the verified implementation (whose output is guaranteed to be correct)
 of the approach by Ailamazyan et al.
 - `test_ranf.sh` - script to test the optimization of RANF queries
 and their translation to SQL by comparing PostgreSQL, MySQL, SQLite, and VeriMon
-- `cnt.py` - script for converting an SQL query Q produced by *radb*
-into an SQL query computing the *query cost* of Q.
+(which is verified and thus its output is guaranteed to be correct)
+- `cnt.py` - script converting an SQL query produced by *radb*
+into an SQL query computing its *query cost*
 - `functions.sh` - helper bash functions
 - `amazon/` - contains scripts for experiments in Figure 7
 - `examples/` - example queries from this README
@@ -52,8 +61,8 @@ and for checking the translation's correctness and Data Golf properties
 Further tools:
 
 - `ailamazyan/` - our implementation of the approach by Ailamazyan et al.,
-including the formally verified core (`verified.ml`)
-and the underlying theories (in subdirectory `thys`)
+including the formally verified core (`src/verified.ml`)
+and the underlying theories (in subdirectory `thys/`)
 - `dddlib/` - the implementation of Difference Decision Diagrams (DDD)
 - `ddd-rc/` - our implementation of a tool using DDDs for evaluating RC queries
 - `ldd-r6438/` - the implementation of Linear Decision Diagrams (LDD)
@@ -70,7 +79,7 @@ We recommend running the experiments using `docker` and the provided `Dockerfile
 Please set up at least 8 GiB of main memory for your Docker container.
 Note that the first command below will take some time to finish (roughly 20 minutes).
 ```
-sudo docker build -t rc2sql .
+sudo docker build --no-cache -t rc2sql .
 sudo docker run -it rc2sql
 ```
 Once you run the second command above you will
@@ -84,7 +93,20 @@ Hence, we set `enable_nestloop = off` in all our experiments (l. 77 in Dockerfil
 
 # Usage
 
-To run RC2SQL type:
+To evaluate an RC query using RC2SQL and a database engine `${db}` type:
+
+```
+
+$ ./eval_${db}.sh ${prefix}
+
+```
+
+where
+
+prefix = prefix of the path to a text file with an RC query (`${prefix}.fo`),
+a training database (`${prefix}.tdb`), and the actual database (`${prefix}.db`).
+
+To run our translation RC2SQL (without evaluating the query on an actual database) type:
 
 ```
 
@@ -92,7 +114,7 @@ $ ./src/rtrans.native ${prefix}
 
 ```
 
-and to run VGTrans type:
+and to run the translation VGTrans (without evaluating the query on an actual database) type:
 
 ```
 $ ./src/vgtrans.native ${prefix}
@@ -100,14 +122,14 @@ $ ./src/vgtrans.native ${prefix}
 
 where
 
-prefix  = prefix of the path to a text file with an RC query (`${prefix}.fo`)
-and training database (`${prefix}.tdb`).
+prefix = prefix of the path to a text file with an RC query (`${prefix}.fo`)
+and a training database (`${prefix}.tdb`).
 
 RC2SQL outputs a pair of queries (`${prefix}.afin`, `${prefix}.ainf`) using
 the optimizations and a pair of queries (`${prefix}.sfin`, `${prefix}.sinf`)
 without optimizations.
 
-VGTrans outputs queries of the form `${prefix}.v{afin, ainf, sfin, sinf}`.
+VGTrans outputs the queries `${prefix}.v{afin, ainf, sfin, sinf}`.
 
 RC Syntax
 
@@ -131,7 +153,8 @@ RC Syntax
 ```
 
 where `{NUM}` is a nonnegative integer (constant)
-and `{ID}` is an identifier (variable).
+and `{ID}` is an identifier (variable) consisting
+of alphanumeric characters.
 Non-terminals are enclosed in curly braces.
 
 Database Syntax
@@ -160,14 +183,14 @@ It is not an error and can safely be ignored.
 
 The script contains example invocations of all the tools used in the artifact.
 
-The script creates a random query using the tool `./tools/gen_test`. (You can invoke the tool without any arguments to see its usage.)
-Then the script translates the query to RANF queries using RC2SQL and VGTrans tools and then to SQL using the *radb* tool. It creates both optimized and unoptimized translations.
+The script creates a random query using the tool `./tools/gen_test`. (You can invoke the tool without any arguments to display its usage.)
+Then the script translates the query to RANF queries using the RC2SQL and VGTrans tools and then to SQL using the *radb* tool. It creates both optimized and unoptimized translations.
 
-It then sets up PostgreSQL and MySQL databases to contain an example database and evaluates the queries using Verimon, PostgreSQL, MySQL, tool by Ailamazyan et al, DDDs, LDDs, and MonPoly-Reg.
-Results of the evaluation of all tools are then compared to the expected result provided by the Ailamazyan et al.'s tool (hence the "OK"s in the output).
+Then it sets up PostgreSQL and MySQL databases to contain an example database and evaluates the queries using Verimon, PostgreSQL, MySQL, tool by Ailamazyan et al, DDDs, LDDs, and MonPoly-Reg.
+Results of the evaluation using all tools are then compared to the expected result provided by the Ailamazyan et al.'s tool (hence the "OK"s in the output).
 
-Finally it computes the cost of each translated query using the `cnt.py` script.
-Hence the output of the form:
+Finally the script computes the cost of each translated query using the `cnt.py` script.
+Hence, it produces output of the form:
 
 ```
  cost
@@ -204,7 +227,7 @@ $ ./run.sh
 
 The individual experiments are described in Section 5.
 After the script `run.sh` finishes,
-the results are contained in the files `exps*.tex`
+the results are contained in the files `exps_*.tex`
 used to plot Figure 6 and 7.
 
 A PDF with the evaluation results can be obtained by executing
@@ -214,12 +237,12 @@ $ pdflatex main.tex
 ```
 
 The timeout for the individual experiments can be set
-in the scripts `exps*.sh`. With the unmodified timeouts of 300s and 600s, respectively,
+in the scripts `exps_*.sh`. With the unmodified timeouts of 300s and 600s, respectively,
 the script would take overnight to recreate the tables.
 
 Note. If you want to run the benchmarks with a tool
 that is omitted in the paper because the tool always times out or crashes,
-please uncomment the corresponding line in the script `exps*.sh`, e.g.,
+please uncomment the corresponding line in the script `exps_*.sh`, e.g.,
 to execute LDDs in the experiment LARGE, uncomment the following line
 ```
 #line "\\ldd" run04LDD
@@ -285,7 +308,8 @@ Please refer to the `README.md` file in the folder `nf/` for more details.
 
 Running `for i in {0..9}; do ./test_ranf.sh 14 4 2 1 10 2 1 ${i}; done`
 tests the translation of the queries used in the SMALL experiment
-from RANF to SQL by comparing PostgreSQL, MySQL, SQLite, and VeriMon.
+from RANF to SQL by comparing PostgreSQL, MySQL, SQLite, and VeriMon
+(which is verified and thus its output is guaranteed to be correct).
 Here we use `n = 10` as the script `test_ranf.sh` cannot be used with a higher value of the parameter `n`.
 
 The output (in the file `log.txt`)
@@ -306,7 +330,7 @@ produced by VGT (prefix `v`).
 `DIFF(p-v)` denotes an output inconsistency between PostgreSQL and VeriMon.
 `DIFF(v-v)` denotes an output inconsistency between optimized and unoptimized RANF queries.
 `DIFF(dg)` denotes a violation of Data Golf properties (positive set is not contained
-in the result or negative set has a nonempty intersection with the result)
+in the result or negative set has nonempty intersection with the result)
 
 Note. We remark that the output of MySQL can be nondeterministic, i.e.,
 some of the above inconsistencies might not be reported at every execution
@@ -320,7 +344,7 @@ To test RC2SQL/VGTrans against the formally verified implementation
 of the approach by Ailamazyan et al. run
 
 ```
-$ ./run_tests.sh
+$ ./test_all.sh
 ```
 
 In total, 40 tests are executed (they take roughly 5 minutes to finish).
@@ -328,7 +352,7 @@ The errors are printed into `log.txt` (the file does not exist if no error
 has been found).
 The tests are conducted on pseudorandom queries and databases.
 The parameters are summarized here and can be easily adjusted in the file
-`run_tests.sh`.
+`test_all.sh`.
 
 - Number of subqueries: 10
 - Maximum arity of a subquery: 4
@@ -342,8 +366,7 @@ The parameters are summarized here and can be easily adjusted in the file
 
 # Formalization of the approach by Ailamazyan et al. in Isabelle/HOL
 
-The formal development can be browsed as a generated HTML page
-(open `ailamazyan/html/index.html`).
+The formal development can be browsed as a generated HTML page (open `ailamazyan/html/index.html`).
 An alternative way to study the theory files is to open them in Isabelle/jEdit.
 
 The raw Isabelle sources are included in the directory `ailamazyan/thys`.
@@ -352,19 +375,35 @@ The formalization can been processed with the development version of Isabelle, w
 
 https://isabelle-dev.sketis.net/source/isabelle/
 
-and the development version of AFP, which can be downloaded from
+and installed following the standard instructions from
+
+https://isabelle-dev.sketis.net/source/isabelle/browse/default/README_REPOSITORY
+
+The formalization has been tested with changeset 74363:383fd113baae of Isabelle:
+```
+$ isabelle/Admin/init -r 383fd113baae
+```
+
+It also requires the development version of the Archive of Formal Proofs, which can be downloaded from
 
 https://isabelle-dev.sketis.net/source/afp-devel/
 
-To build the theories, export the verified OCaml code,
-and regenerate the HTML page, run
-`isabelle build -d '$AFP' -o browser_info -c -e -v -D thys/`
-in the directory `ailamazyan/`.
+and installed following the standard instructions from
+
+https://www.isa-afp.org/using.html
+
+The formalization has been tested with changeset 12040:61b65f5bfdbe of AFP:
+```
+$ hg update -r 61b65f5bfdbe
+```
+
+To build the theories, export the verified OCaml code, and regenerate the HTML page, run
+`isabelle build -o browser_info -c -e -v -D thys`
+in the directory `ailamazyan`.
 This should take roughly 20 minutes.
-Instructions where to find the verified OCaml code
-and the generated html sources are printed in the console.
+Instructions where to find the verified OCaml code and the generated html sources are printed in the console.
 
 To build the pdf document, run
-`~/isabelle/bin/isabelle document -d '$AFP' -d thys/ -O thys/ -v Eval_FO`
-in the directory `ailamazyan/`.
+`isabelle document -d thys -O thys -v Eval_FO`
+in the directory `ailamazyan`.
 Instructions where to find the pdf document are printed in the console.
