eval_psql.sh
@@ -1,0 +1,12 @@
+PREFIX="${1}"
+ABS="$(readlink -m "$(dirname "${PREFIX}")")"/"$(basename "${PREFIX}")"
+
+/home/rcsql/src/rtrans.native "${ABS}"
+
+/home/rcsql/tools/db2csv "${ABS}"
+
+/home/rcsql/radb.sh "${ABS}"
+
+psql < "${ABS}.psql" &> /dev/null
+
+/home/rcsql/run_psql.sh "${ABS}.a"
