eval_vmon.sh
@@ -1,0 +1,13 @@
+PREFIX="${1}"
+ABS="$(readlink -m "$(dirname "${PREFIX}")")"/"$(basename "${PREFIX}")"
+
+grep -o "[A-Za-z0-9]*([A-Za-z0-9, ]*)" "${ABS}.fo" | sed "s/[A-Za-z0-9]* *,/int,/g" | sed "s/[A-Za-z0-9]* *)/int)/g" > "${ABS}.sig"
+echo "@0 " > "${ABS}.log"
+cat "${ABS}.db" >> "${ABS}.log"
+
+/home/rcsql/src/rtrans.native "${ABS}"
+
+. /home/rcsql/functions.sh
+symlinks "${ABS}"
+
+/home/rcsql/run_vmon.sh "${ABS}.a"
