examples/ex.sh
@@ -1,5 +1,9 @@
 ./tools/gen_test /home/rcsql/examples/ex 8 4 2 1 10 10 0 0 # 1st argument of gen_test must be ABSOLUTE path
 
+./eval_vmon.sh examples/ex > examples/ex.eoa
+./eval_psql.sh examples/ex > examples/ex.eopa
+./eval_msql.sh examples/ex > examples/ex.eoma
+
 ./src/rtrans.native examples/ex
 
 ./src/vgtrans.native examples/ex
@@ -12,18 +16,21 @@ symlinks /home/rcsql/examples/ex # 1st argument of symlinks must be ABSOLUTE pat
 psql < examples/ex.psql
 mysql -u rcsql --local-infile=1 < examples/ex.msql
 
-./rw_vmon.sh examples/ex.a > examples/ex.oa    # RC2SQL
-./rw_vmon.sh examples/ex.s > examples/ex.os    # RC2SQL*
-./rw_vmon.sh examples/ex.va > examples/ex.ova  # VGTrans
-./rw_vmon.sh examples/ex.vs > examples/ex.ovs  # VGTrans*
-./rw_psql.sh examples/ex.a > examples/ex.opa   # RC2SQL
-./rw_psql.sh examples/ex.s > examples/ex.ops   # RC2SQL*
-./rw_psql.sh examples/ex.va > examples/ex.opva # VGTrans
-./rw_psql.sh examples/ex.vs > examples/ex.opvs # VGTrans*
-./rw_msql.sh examples/ex.a > examples/ex.oma   # RC2SQL
-./rw_msql.sh examples/ex.s > examples/ex.oms   # RC2SQL*
-./rw_msql.sh examples/ex.va > examples/ex.omva # VGTrans
-./rw_msql.sh examples/ex.vs > examples/ex.omvs # VGTrans*
+./run_vmon.sh examples/ex.a > examples/ex.oa    # RC2SQL
+diff examples/ex.oa examples/ex.eoa
+./run_vmon.sh examples/ex.s > examples/ex.os    # RC2SQL*
+./run_vmon.sh examples/ex.va > examples/ex.ova  # VGTrans
+./run_vmon.sh examples/ex.vs > examples/ex.ovs  # VGTrans*
+./run_psql.sh examples/ex.a > examples/ex.opa   # RC2SQL
+diff examples/ex.opa examples/ex.eopa
+./run_psql.sh examples/ex.s > examples/ex.ops   # RC2SQL*
+./run_psql.sh examples/ex.va > examples/ex.opva # VGTrans
+./run_psql.sh examples/ex.vs > examples/ex.opvs # VGTrans*
+./run_msql.sh examples/ex.a > examples/ex.oma   # RC2SQL
+diff examples/ex.oma examples/ex.eoma
+./run_msql.sh examples/ex.s > examples/ex.oms   # RC2SQL*
+./run_msql.sh examples/ex.va > examples/ex.omva # VGTrans
+./run_msql.sh examples/ex.vs > examples/ex.omvs # VGTrans*
 
 ./ailamazyan/src/ail.native -fmla examples/ex.fo -db examples/ex.db > examples/ex.ail # Ailamazyan et al.
 ./ddd-rc/ddd examples/ex.fo examples/ex.db > examples/ex.ddd # DDD
@@ -61,7 +68,7 @@ python3 cnt.py examples/ex.vspsqlinf | psql
 python3 cnt.py examples/ex.vsmsqlfin | sed "s/WITH/USE db;\nWITH/" | mysql -u rcsql
 python3 cnt.py examples/ex.vsmsqlinf | sed "s/WITH/USE db;\nWITH/" | mysql -u rcsql
 
-./test_rw.sh 8 4 2 1 10 10 0 0
+./test_eval.sh 8 4 2 1 10 10 0 0
 ./test_ranf.sh 8 4 2 1 10 10 0 0
 
 cat log.txt # the file should only exist if there are errors
