run.sh
@@ -1,11 +1,9 @@
 . ./functions.sh
 
-seeds="0 1 2 3 4 5 6 7 8 9"
-
 ./exps_small.sh 14 4 2 1 500 2 "0 1 2 3 4 5 6 7 8 9" > exps_small.tex
 ./exps_medium.sh 14 4 2 1 20000 2 "0 1 2 3 4 5 6 7 8 9" > exps_medium.tex
 ./exps_large.sh 14 4 2 1 "40000 80000 120000" 2 "0 1 2 3 4 5 6 7 8 9" > exps_large.tex
-./exps_inf.sh 0 4 2 0 4000 2 "14 30 64 108 190 15 31 65 109 191" > exps_inf.tex
+./exps_inf.sh 0 4 2 0 4000 2 "14 30 64 108 184 15 31 65 109 185" > exps_inf.tex
 ./exps_susp.sh > exps_susp.tex
 
 #./bold.sh
