test_all.sh
@@ -4,7 +4,7 @@ do
   do
     for k in {0..1}
     do
-      ./test_rw.sh 10 4 2 ${k} 4 2 ${j} ${i}
+      ./test_eval.sh 10 4 2 ${k} 4 2 ${j} ${i}
     done
   done
 done
